examples/tactics/UserTactics.fst
@@ -61,8 +61,10 @@ assume val mul_comm : x:nat -> y:nat -> Tot (op_Multiply x y == op_Multiply y x)
 val lemma_mul_comm : x:nat -> y:nat -> Lemma (op_Multiply x y == op_Multiply y x)
 let lemma_mul_comm x y = ()
 
+let sqintro (x:'a) : squash 'a = ()
+
 let test_exact (x:nat) (y:nat) =
-  assert_by_tactic (exact (quote (mul_comm x y)))
+  assert_by_tactic (exact (quote (sqintro (mul_comm x y))))
                    (op_Multiply x y == op_Multiply y x)
 
 let test_apply (x:nat) (y:nat) =
@@ -115,11 +117,11 @@ let test_simpl =
                       let (e, g), _ = eg in
                       (match term_as_formula g with
                       | And _ _ -> return ()
-                      | _ -> fail "not a conjunction?");;
+                      | _ -> dump "not a conjunction?");;
                       simpl;;
                       eg <-- cur_goal;
                       let (e, g), _ = eg in
                       (match term_as_formula g with
                       | True_ -> return ()
-                      | _ -> fail ("not true after simpl? " ^ term_to_string g)))
+                      | _ -> dump ("not true after simpl? " ^ term_to_string g)))
                      (True /\ 1 == 1)
